Weidenbach_Book/IsaSAT_Initialisation.thy
@@ -422,8 +422,8 @@ lemma add_init_cls_heur_add_init_cls:
 definition (in isasat_input_ops) already_propagated_unit_cls_conflict
   :: \<open>nat literal \<Rightarrow> nat twl_st_wl_init \<Rightarrow> nat twl_st_wl_init\<close>
 where
-  \<open>already_propagated_unit_cls_conflict = (\<lambda>L ((M, N, U, D, NE, UE, Q, WS), OC).
-     ((M, N, U, D, add_mset {#L#} NE, UE, {#}, WS), OC))\<close>
+  \<open>already_propagated_unit_cls_conflict = (\<lambda>L ((M, N, D, NE, UE, Q, WS), OC).
+     ((M, N, D, add_mset {#L#} NE, UE, {#}, WS), OC))\<close>
 
 definition (in isasat_input_ops) already_propagated_unit_cls_conflict_heur
   :: \<open>nat literal \<Rightarrow> twl_st_wl_heur_init \<Rightarrow> twl_st_wl_heur_init nres\<close>
