Weidenbach_Book/IsaSAT_Lookup_Conflict.thy
@@ -563,10 +563,6 @@ where
      lookup_conflict_merge zero_uint32_nat M (C\<propto>i) xs clvls lbd outl\<close>
 
 (* TODO Move *)
-lemma(in isasat_input_ops) in_\<L>\<^sub>a\<^sub>l\<^sub>l_atm_of_\<A>\<^sub>i\<^sub>n:
-  \<open>xa \<in># \<L>\<^sub>a\<^sub>l\<^sub>l \<longleftrightarrow> atm_of xa \<in># \<A>\<^sub>i\<^sub>n\<close>
-  by (simp add: atms_of_\<L>\<^sub>a\<^sub>l\<^sub>l_\<A>\<^sub>i\<^sub>n in_\<L>\<^sub>a\<^sub>l\<^sub>l_atm_of_in_atms_of_iff)
-
 lemma (in isasat_input_ops) literals_are_in_\<L>\<^sub>i\<^sub>n_trail_atm_of:
   \<open>literals_are_in_\<L>\<^sub>i\<^sub>n_trail M \<longleftrightarrow> atm_of ` lits_of_l M \<subseteq> set_mset \<A>\<^sub>i\<^sub>n\<close>
   apply (rule iffI)
