Weidenbach_Book/Watched_Literals_Watch_List_Domain.thy
@@ -543,6 +543,83 @@ proof -
        learned_clss.simps init_clss.simps)
 qed
 *)
+
+lemma in_\<L>\<^sub>a\<^sub>l\<^sub>l_atm_of_\<A>\<^sub>i\<^sub>n:\<open>L \<in># \<L>\<^sub>a\<^sub>l\<^sub>l \<longleftrightarrow> atm_of L \<in># \<A>\<^sub>i\<^sub>n\<close>
+  by (cases L) (auto simp: \<L>\<^sub>a\<^sub>l\<^sub>l_def)
+
+lemma literals_are_in_\<L>\<^sub>i\<^sub>n_alt_def:
+  \<open>literals_are_in_\<L>\<^sub>i\<^sub>n S \<longleftrightarrow> atms_of S \<subseteq> atms_of \<L>\<^sub>a\<^sub>l\<^sub>l\<close>
+  apply (auto simp: literals_are_in_\<L>\<^sub>i\<^sub>n_def all_lits_of_mm_union lits_of_def
+       in_all_lits_of_m_ain_atms_of_iff in_all_lits_of_mm_ain_atms_of_iff atms_of_\<L>\<^sub>a\<^sub>l\<^sub>l_\<A>\<^sub>i\<^sub>n
+       atm_of_eq_atm_of uminus_\<A>\<^sub>i\<^sub>n_iff subset_iff in_\<L>\<^sub>a\<^sub>l\<^sub>l_atm_of_\<A>\<^sub>i\<^sub>n)
+  apply (auto simp: atms_of_def)
+  done
+
+lemma
+  assumes
+      x2_T: \<open>(x2, T) \<in> state_wl_l None\<close> and
+      struct: \<open>twl_struct_invs U\<close> and
+      T_U: \<open>(T, U) \<in> twl_st_l None\<close>
+  shows
+    literals_are_\<L>\<^sub>i\<^sub>n_literals_are_\<L>\<^sub>i\<^sub>n_trail:
+      \<open>literals_are_\<L>\<^sub>i\<^sub>n x2 \<Longrightarrow> literals_are_in_\<L>\<^sub>i\<^sub>n_trail (get_trail_wl x2)\<close> 
+     (is \<open>_\<Longrightarrow> ?trail\<close>) and
+    literals_are_\<L>\<^sub>i\<^sub>n_literals_are_in_\<L>\<^sub>i\<^sub>n_conflict:
+      \<open>literals_are_\<L>\<^sub>i\<^sub>n x2 \<Longrightarrow> get_conflict_wl x2 \<noteq> None \<Longrightarrow> literals_are_in_\<L>\<^sub>i\<^sub>n (the (get_conflict_wl x2))\<close> and
+    conflict_not_tautology:
+      \<open>get_conflict_wl x2 \<noteq> None \<Longrightarrow> \<not>tautology (the (get_conflict_wl x2))\<close>
+proof -
+  have 
+    alien: \<open>cdcl\<^sub>W_restart_mset.no_strange_atm (state\<^sub>W_of U)\<close> and
+    confl: \<open>cdcl\<^sub>W_restart_mset.cdcl\<^sub>W_conflicting (state\<^sub>W_of U)\<close> and
+    M_lev: \<open>cdcl\<^sub>W_restart_mset.cdcl\<^sub>W_M_level_inv (state\<^sub>W_of U)\<close> and
+    dist: \<open>cdcl\<^sub>W_restart_mset.distinct_cdcl\<^sub>W_state (state\<^sub>W_of U)\<close>
+   using struct unfolding twl_struct_invs_def cdcl\<^sub>W_restart_mset.cdcl\<^sub>W_all_struct_inv_def
+   by fast+
+
+  show lits_trail: \<open>literals_are_in_\<L>\<^sub>i\<^sub>n_trail (get_trail_wl x2)\<close>
+    if \<open>literals_are_\<L>\<^sub>i\<^sub>n x2\<close>
+    using alien that x2_T T_U unfolding is_\<L>\<^sub>a\<^sub>l\<^sub>l_def
+      literals_are_in_\<L>\<^sub>i\<^sub>n_trail_def cdcl\<^sub>W_restart_mset.no_strange_atm_def
+    by (subst (asm) all_clss_l_ran_m[symmetric])
+      (auto simp add: twl_st twl_st_l twl_st_wl all_lits_of_mm_union lits_of_def
+        convert_lits_l_def image_image in_all_lits_of_mm_ain_atms_of_iff
+        get_unit_clss_wl_alt_def
+        simp del: all_clss_l_ran_m)
+
+  {
+    assume conf: \<open>get_conflict_wl x2 \<noteq> None\<close>
+    show lits_confl: \<open>literals_are_in_\<L>\<^sub>i\<^sub>n (the (get_conflict_wl x2))\<close>
+      if \<open>literals_are_\<L>\<^sub>i\<^sub>n x2\<close>
+      using x2_T T_U alien that conf unfolding is_\<L>\<^sub>a\<^sub>l\<^sub>l_alt_def
+       cdcl\<^sub>W_restart_mset.no_strange_atm_def literals_are_in_\<L>\<^sub>i\<^sub>n_alt_def
+      apply (subst (asm) all_clss_l_ran_m[symmetric])
+     unfolding image_mset_union all_lits_of_mm_union
+      by (auto simp add: twl_st twl_st_l twl_st_wl all_lits_of_mm_union lits_of_def
+         image_image in_all_lits_of_mm_ain_atms_of_iff
+        in_all_lits_of_m_ain_atms_of_iff
+        get_unit_clss_wl_alt_def
+        simp del: all_clss_l_ran_m)
+
+    have M_confl: \<open>get_trail_wl x2 \<Turnstile>as CNot (the (get_conflict_wl x2))\<close>
+      using confl conf x2_T T_U unfolding cdcl\<^sub>W_restart_mset.cdcl\<^sub>W_conflicting_def
+      by (auto 5 5 simp: twl_st twl_st_l true_annots_def)
+    moreover have n_d: \<open>no_dup (get_trail_wl x2)\<close>
+      using M_lev x2_T T_U unfolding cdcl\<^sub>W_restart_mset.cdcl\<^sub>W_M_level_inv_def
+      by (auto simp: twl_st twl_st_l)
+    ultimately show 4: \<open>\<not>tautology (the (get_conflict_wl x2))\<close>
+      using n_d M_confl
+      by (meson no_dup_consistentD tautology_decomp' true_annots_true_cls_def_iff_negation_in_model)
+  }
+qed
+
+lemma (in isasat_input_ops) literals_are_in_\<L>\<^sub>i\<^sub>n_trail_atm_of:
+  \<open>literals_are_in_\<L>\<^sub>i\<^sub>n_trail M \<longleftrightarrow> atm_of ` lits_of_l M \<subseteq> set_mset \<A>\<^sub>i\<^sub>n\<close>
+  apply (rule iffI)
+  subgoal by (auto dest: literals_are_in_\<L>\<^sub>i\<^sub>n_trail_in_lits_of_l_atms)
+  subgoal by (fastforce simp: literals_are_in_\<L>\<^sub>i\<^sub>n_trail_def lits_of_def in_\<L>\<^sub>a\<^sub>l\<^sub>l_atm_of_\<A>\<^sub>i\<^sub>n)
+  done
+
 end
 
 
